theories/OptionBind.v
@@ -1,0 +1,6 @@
+Definition option_bind {A B} : (A -> option B) -> option A -> option B := fun f opt =>
+  match opt with
+  | None => None
+  | Some x => f x
+  end.
+Arguments option_bind {A B} f/ opt.
